language_formal/spark2014_semantics/propertyProof.v
@@ -12,7 +12,6 @@ zhangzhi@ksu.edu
 Require Export util.
 Require Export wellformedness.
 Require Export semantics.
-Require Export typing.
 
 (** * Properties Proof *)
 
